\renewcommand{\theequation}{\theenumi}

\begin{enumerate}[label=\arabic*.,ref=\thesubsection.\theenumi]
		\numberwithin{equation}{enumi}

	\item If $s1 \ne s_2$ are in $S$, show that there is an $f \in A(S)$ such that $f(s_1) = s_2$.
		\\
		\solution By definition of a 1-1 mapping, it is obvious.
	\item If $s_1 \in S$, let $H = \cbrak{f \in A(S) \mid f(s_1) = s_1}$. Show that: 
		\label{prob:1.4.2}
		\begin{enumerate}
		\item  $i \in H$. 
		\item  If $f, g \in H$, then $fg \in H$. 
		\item  If $f \in H$, then $f^{-1} \in H$.
		\end{enumerate}
		\solution 
		\begin{enumerate}
			\item $\because i(s_1) = s_1, i \in H$.
			\item $fg(s_1)= f(s_1) = s_1.$
			\item $f(s_1) = s_1 \implies f^{-1}(s_1) = s_1 \implies f^{-1} \in H$.
		\end{enumerate}
	\item Suppose that $s_1 \ne s_2$ are in $S$ and $f(s_1) = s_2$, where $f \in A (S)$. Then if $H$ is as in Problem
		\ref{prob:1.4.2}
		 and $K = \cbrak{g \in A (S) \mid g(s_2) = s_2}$, show that:
\begin{enumerate}
	\item  If $g \in K$, then $f^{-1}gf \in H$. 
	\item  If $h \in H$, then there is some $g \in K$ such that $h = f^{-1}gf$.
\end{enumerate}
\solution
\begin{enumerate}
	\item  From the given information,
		\begin{align}
			f^{-1}gf(s_1) =  
			f^{-1}g(s_2) =   
			f^{-1}(s_2) =  s_1 
		\end{align}
		Hence, 
		\begin{align}
			f^{-1}gf  \in H 
		\end{align}
	\item  The $h$ was found in the previous part.
\end{enumerate}
\item If $f, g, h \in A(S)$, show that $(f^{-1}gf)(f^{-1}hf) = f^{-1}(gh)f$. What can you say about $(f^{-1}gf)^n$?
\solution  From the given information, 
		\begin{align}
			(f^{-1}gf)(f^{-1}hf) &= 
			f^{-1}g\brak{ff^{-1}}hf 
\\
			&			= 
			f^{-1}\brak{gh}f  
		\end{align}
		Similarly,
		\begin{align}
			\brak{f^{-1}gf}^n = 
			f^{-1}g^n  f
		\end{align}
	\item If $f, g \in A (S)$ and $fg = gf$, show that:
\begin{enumerate}
	\item  $(fg)^2 = f^2g^2$.
	\item  $(fg)^{-1} = f^{-1g^{-1}}$.
\end{enumerate}
\solution From the given information, 
\begin{enumerate}
	\item  
		\begin{align}
			(fg)^2 &= \brak{fg}\brak{fg}
			\\
			 &= \brak{fg}\brak{gh} = fg^2h
		\begin{align}
	\item  $(fg)^{-1} = f^{-1g^{-1}}$.
\end{enumerate}
\end{enumerate}
